Defined hoare' etc (variants of hoare etc that work outside a proof)

Test.thy
@@ -4,57 +4,45 @@ begin
 
 ML_file "test.ML"
 
-lemma True
+program' (demo_logic) prog: \<open>[Set STR ''x'' 5, Guess STR ''y'', Add STR ''x'' STR ''y'']\<close>
+
+(* TODO: should be handled by program-command *)
+definition prog where "prog = [Set STR ''x'' 5, Guess STR ''y'', Add STR ''x'' STR ''y'']"
+
+invariant' (demo_logic) start: "\<lambda>m. True"
+
+lemma "hoare start_inv prog (\<lambda>m. m STR ''x'' = 0)"
 proof  -
-
-  program (demo_logic) prog: \<open>[Set STR ''x'' 5, Guess STR ''y'', Add STR ''x'' STR ''y'']\<close>
-
-  (* TODO: should be handled by program-command *)
-  define prog where "prog = [Set STR ''x'' 5, Guess STR ''y'', Add STR ''x'' STR ''y'']"
-
-  invariant (demo_logic) start: "\<lambda>m. True"
 
   (* Step 1: Set x 5 *)
 
-  (* invariant (demo_logic) step1: \<open>(postcondition_trivial (Set STR ''x'' 5) start_inv)\<close> *)
-
-(* TODO: step1 should be defined by this *)
-  hoare step1: range 0-1 pre start post step1=trivial
-(*   do_prf \<open>Forward_Hoare.new_hoare_auto \<^binding>\<open>step1\<close> fst (Forward_Hoare.get_current_program \<^context> |> the)
-            (Demo_Hoare.ex_range (0,1)) "start" \<^binding>\<open>step1\<close> "trivial"\<close> *)
-    by -
+  hoare step1: range 0-1 pre start post step1=trivial.
 
   invariant_has step1_x5: step1 \<rightarrow> "\<lambda>m. m STR ''x'' = 5"
     using step1_inv_def by (rule newvalue)
 
   (* Step 2: Guess y *)
 
-  (* invariant (demo_logic) step2: \<open>postcondition_pick (Guess STR ''y'') (-5) step1_inv\<close> *)
-  hoare step2: extends step1 range 1-2 post step2=pick -5
-    by -
-
-(*   do_prf \<open>Forward_Hoare.extend_hoare_auto \<^binding>\<open>step2\<close> "step1" #1 (Demo_Hoare.ex_range (1,2))
- \<^binding>\<open>step2\<close> "pick" (Token.explode0 Keyword.empty_keywords "-5")\<close>
-    by - *)
+  hoare step2: extends step1 range 1-2 post step2=pick -5.
 
   invariant_has step2_x5: step2 \<rightarrow> "\<lambda>m. m STR ''x'' = 5"
+
     using step2_inv_def apply (rule unchanged)
      apply (rule independent_ofI, simp)
     apply (tactic \<open>Demo_Hoare.use_facts_tac \<^context> @{thms step1_x5} 1\<close>)
     by simp
 
   invariant_has step2_y5: step2 \<rightarrow> "\<lambda>m. m STR ''y'' = -5"
+
     using step2_inv_def by (rule newvalue)
 
   (* Step 3: Add x y *)
 
-  (* invariant (demo_logic) step3: \<open>(postcondition_trivial (Add STR ''x'' STR ''y'') step2_inv)\<close> *)
   hoare step3: extends step2 range 2-3 post step3=trivial
-(*   do_prf \<open>Forward_Hoare.extend_hoare_auto \<^binding>\<open>step3\<close> "step2" #1 (Demo_Hoare.ex_range (2,3)) 
-    \<^binding>\<open>step3\<close> "trivial" []\<close> *)
     by auto
 
   invariant_has step3_y5: step3 \<rightarrow> "\<lambda>m. m STR ''y'' = -5"
+
     using step3_inv_def apply (rule unchanged)
       apply (rule independent_ofI, simp)
      apply simp
@@ -62,20 +50,20 @@ proof  -
     by simp
 
   invariant_has step3_x0: step3 \<rightarrow> "\<lambda>m. m STR ''x'' = 0"
+
     using step3_inv_def apply (rule wp)
      apply simp
     apply (tactic \<open>Demo_Hoare.use_facts_tac \<^context> @{thms step2_x5 step2_y5} 1\<close>)
     by simp
 
   from step3_valid
-  have "hoare (\<lambda>_. True) prog (\<lambda>m. m STR ''x'' = 0)"
+  show ?thesis
     unfolding prog_def
     apply (rule hoare_conseq')
-    unfolding start_inv_def apply (simp add: pc_imp_def)
+      apply (simp add: pc_imp_def)
      apply (rule step3_x0)
     by simp
 
-  show ?thesis by simp
 qed
 
 end
